vale/code/arch/Vale.Arch.Heap.fst
@@ -13,17 +13,18 @@ let heap_taint hi = hi.vf_layout.vl_taint
 
 let heap_upd hi mh' mt' =
   let h' = mi_heap_upd hi.vf_heap mh' in
+  let hh' = ValeHeap h'.mh h'.ih (Map16.sel hi.vf_heaplets 0).heapletId in
   {
     vf_layout = {hi.vf_layout with vl_taint = mt'};
     vf_heap = h';
-    vf_heaplets = Map16.upd hi.vf_heaplets 0 h';
+    vf_heaplets = Map16.upd hi.vf_heaplets 0 hh';
   }
 
 let heap_create_machine ih =
   down_mem ih
 
 let heap_create_impl ih mt =
-  let vh = ValeHeap (down_mem ih) (Ghost.hide ih) in
+  let vh = ValeHeap (down_mem ih) (Ghost.hide ih) None in
   let vh4 = ((vh, vh), (vh, vh)) in
   let vh16 = ((vh4, vh4), (vh4, vh4)) in
   let layout_inner = {
